FokkerChallenge/EnhancedCslib/LeftMost.lean
@@ -1,0 +1,30 @@
+import Cslib.Languages.LambdaCalculus.LocallyNameless.Untyped.Basic
+import Cslib.Languages.LambdaCalculus.LocallyNameless.Untyped.LcAt
+import Cslib.Languages.LambdaCalculus.LocallyNameless.Untyped.LeftmostReduction
+import Cslib.Foundations.Data.HasFresh
+import FokkerChallenge.Basic
+import Mathlib.Data.Finset.Basic
+import Mathlib.Data.Finset.Insert
+import Mathlib.Data.Finset.Union
+
+namespace Cslib
+
+namespace LambdaCalculus.LocallyNameless.Untyped.Term
+
+theorem leftmost_multiapp (f a: Term String) (l) : f.abs.LC -> a.LC ->
+  (a :: l).foldl Term.app f.abs ⭢ℓ l.foldl Term.app (f^a) := by
+  induction l using List.reverseRecOn generalizing f a with
+  | nil => apply BetaAt.outer
+  | append_singleton l a _ => intros _ _
+                              simp
+                              apply BetaAt.appNoAbsL
+                              grind
+                              intros h
+                              generalize heq : (List.foldl app (f.abs.app a) l) = Q
+                              rw [heq] at h
+                              cases h
+                              induction l using List.reverseRecOn with grind
+
+end LambdaCalculus.LocallyNameless.Untyped.Term
+
+end Cslib
